case_study/MinimalCaps/Contracts.v
@@ -686,6 +686,8 @@ Local Ltac solve :=
        | |- False \/ _ =>  right
        | |- _ \/ False =>  left
        | |- _ /\ _ => constructor
+       | |- VerificationCondition _ => constructor; cbn
+       | |- Obligation _ _ _ => constructor; cbn
        | |- Debug _ _ => constructor
        | |- Debug _ True \/ _ => left
        | |- (_ \/ _) \/ _ =>  rewrite or_assoc
@@ -750,9 +752,7 @@ Lemma valid_contract_upper_bound : ValidContractDynMut sep_contract_upper_bound 
 Proof. apply dynmutevarreflect_sound; reflexivity. Abort.
 
 Lemma valid_contract_within_bounds : ValidContractDynMut sep_contract_within_bounds fun_within_bounds.
-Proof.
-  compute - [sout_safe]; cbn; solve.
-Abort.
+Proof. compute; solve. Abort.
 
 Lemma valid_contract_exec_jr : ValidContractDynMut sep_contract_exec_jr fun_exec_jr.
 Proof. apply dynmutevarreflect_sound; reflexivity. Abort.
